src/proof/k8s_io/apimachinery/pkg/api/meta.v
@@ -1,0 +1,28 @@
+From proof.k8s_io.apimachinery.pkg.api Require Export meta_init.
+From proof.k8s_io.api.core Require Export v1_init.
+From proof Require Import prelude empty_ffi.
+
+Section proof.
+Context `{hG: !heapGS Σ} {go_ctx: GoContext}.
+
+Lemma wp_Accessor i (o: v1.Object.t):
+  {{{ is_pkg_init code.k8s_io.apimachinery.pkg.api.meta.meta ∗
+      "%i_is_Object" ∷ ⌜i = interface.mk v1.Object.id (# o)⌝
+  }}}
+    @! meta.Accessor #i
+  {{{ ret (err: error.t), RET (#ret, #err);
+      ⌜ ret = o ⌝ ∗ ⌜ err = interface.nil ⌝
+  }}}.
+Proof.
+  wp_start as "H". iNamed "H". wp_auto. subst.
+  unshelve wp_apply wp_interface_checked_type_assert; try tc_solve.
+  { iPureIntro. intros Object_id. exists o. done. }
+  iIntros (y ok) "%if_ok".
+  assert (ok = true) as ok_is_true.
+  { destruct ok; [done|]. intuition. }
+  subst ok. inversion if_ok.
+  apply (inj to_val) in H0. subst o.
+  wp_auto. iApply "HΦ". done.
+Qed.
+
+End proof.
