src/proof/k8s_io/apimachinery/pkg/api/meta_init.v
@@ -1,3 +1,5 @@
+From proof Require Export prelude.
+From proof.k8s_io.apimachinery.pkg.apis.meta Require Export v1_init.
 Require Export New.generatedproof.k8s_io.apimachinery.pkg.api.meta.
 
 
