src/proof/k8s_io/apimachinery/pkg/apis/meta/v1.v
@@ -1,0 +1,71 @@
+Require Export New.proof.sync.
+
+From proof.k8s_io.apimachinery.pkg.apis.meta Require Export v1_init.
+From proof.k8s_io.api.core Require Export v1_init.
+From proof Require Import prelude empty_ffi.
+
+Section proof.
+Context `{hG: !heapGS Σ} {go_ctx: GoContext}.
+
+Lemma wp_Now:
+  {{{ is_pkg_init code.k8s_io.apimachinery.pkg.apis.meta.v1.v1 }}}
+    @! v1.Now #()
+  {{{ (v: v1.Time.t), RET #v;
+    True
+  }}}.
+Proof.
+Admitted.
+
+Lemma wp_GetDeletionTimestamp (ptr: loc) (meta: v1.ObjectMeta.t):
+  {{{ is_pkg_init code.k8s_io.apimachinery.pkg.apis.meta.v1.v1 ∗
+      "ptr" ∷ ptr ↦ meta
+  }}}
+    ptr @ (ptrT.id v1.ObjectMeta.id) @ "GetDeletionTimestamp" #()
+  {{{ (deletion_timestamp: loc), RET #deletion_timestamp;
+      ⌜ deletion_timestamp = meta.(v1.ObjectMeta.DeletionTimestamp') ⌝ ∗
+      ptr ↦ meta
+  }}}.
+Proof.
+  wp_start as "H". iNamed "H". wp_auto. iApply "HΦ". iFrame. done.
+Qed.
+
+Lemma wp_SetDeletionTimestamp (ptr: loc) (meta: v1.ObjectMeta.t) (deletion_timestamp: loc):
+  {{{ is_pkg_init code.k8s_io.apimachinery.pkg.apis.meta.v1.v1 ∗
+      "ptr" ∷ ptr ↦ meta
+  }}}
+    ptr @ (ptrT.id v1.ObjectMeta.id) @ "SetDeletionTimestamp" #deletion_timestamp
+  {{{ (meta': v1.ObjectMeta.t), RET #();
+      ⌜ meta' = meta <| v1.ObjectMeta.DeletionTimestamp' := deletion_timestamp |> ⌝ ∗
+      ptr ↦ meta'
+  }}}.
+Proof.
+  wp_start as "H". iNamed "H". wp_auto. iApply "HΦ". iFrame. done.
+Qed.
+
+Lemma wp_SetResourceVersion (ptr: loc) (meta: v1.ObjectMeta.t) (resource_version: go_string):
+  {{{ is_pkg_init code.k8s_io.apimachinery.pkg.apis.meta.v1.v1 ∗
+      "ptr" ∷ ptr ↦ meta
+  }}}
+    ptr @ (ptrT.id v1.ObjectMeta.id) @ "SetResourceVersion" #resource_version
+  {{{ (meta': v1.ObjectMeta.t), RET #();
+      ⌜ meta' = meta <| v1.ObjectMeta.ResourceVersion' := resource_version |> ⌝ ∗
+      ptr ↦ meta'
+  }}}.
+Proof.
+  wp_start as "H". iNamed "H". wp_auto. iApply "HΦ". iFrame. done.
+Qed.
+
+Lemma wp_GetFinalizers (ptr: loc) (meta: v1.ObjectMeta.t):
+  {{{ is_pkg_init code.k8s_io.apimachinery.pkg.apis.meta.v1.v1 ∗
+      "ptr" ∷ ptr ↦ meta
+  }}}
+    ptr @ (ptrT.id v1.ObjectMeta.id) @ "GetFinalizers" #()
+  {{{ (finalizers: slice.t), RET #finalizers;
+      ⌜ finalizers = meta.(v1.ObjectMeta.Finalizers') ⌝ ∗
+      ptr ↦ meta
+  }}}.
+Proof.
+  wp_start as "H". iNamed "H". wp_auto. iApply "HΦ". iFrame. done.
+Qed.
+
+End proof.
